\documentclass{article}
\usepackage{amsmath}

\setlength\parindent{0pt}

\title{Learning Notes on Statistical Learning Theory}
\author{a1trl9}
\date{}

\begin{document}
\maketitle
\section{Lecture 3}
We have achieved:
\begin{equation}
    L(\hat{\theta})-L(\theta^{*}) \approx \frac{p}{2n} + o(\frac{1}{n})
\end{equation}
The limitation of the result above is we assume the data are precisely
distributed according to a particular ground truth parameter \(\theta^{*}\).
Also, we ignore the dependence of higher order terms on other hyperparameters.

\subsection{Uniform Convergence Framework}

\textbf{Definition:} uniform convergence is a property of hypothesis
class \(\mathcal{H}\) of the following form:
\begin{equation}
\mathrm{Pr}[\forall h \in \mathcal{H}, | \hat{L}(\theta)-L(\theta)\leq \epsilon] \geq 1 - \delta
\end{equation}

\textbf{Why uniform convergence framework implies generalization?}
\vspace{2mm}
\begin{equation}
\begin{aligned}
&L(\hat{h})-L(h^{*})\\
&=L(\hat{h}) - \hat{L}(\hat{h})+\hat{L}(\hat{h})-\hat{L}(h^{*})+\hat{L}(h^{*})-L(h^{*})
\end{aligned}
\end{equation}

Since \(\hat{h}\) is the optimal solution for the training example, \(\hat{L}(\hat{h})-\hat{L}(h^{*})\leq 0\), so
we get:
\begin{equation}
\begin{aligned}
L(\hat{h})-L(h^{*})&\leq L(\hat{h}) - \hat{L}(\hat{h})+0+\hat{L}(h^{*})-L(h^{*})\\
&\leq |L(\hat{h})-\hat{L}(\hat{h})| + |\hat{L}(h^*)-L(h^*)|\\
&\leq 2|L({h})-\hat{L}(h)|
\end{aligned}
\end{equation}

Therefore, when uniform convergence holds:
\begin{equation}
\mathrm{Pr}(L(\hat{h})-L(h^{*})\leq 2\epsilon)\geq\mathrm{Pr}[\forall h \in \mathcal{H}, | \hat{L}(\theta)-L(\theta)\leq \epsilon]\geq 1-\delta
\begin{aligned}
\end{aligned}
\end{equation}

\subsection{Finite Hypothesis Classes}
If \(\mathcal(H)\) is finite and \(l(x, y), h)\in [0, 1]\), we have the
following statements (based on Hoeffding Inequality):
\begin{enumerate}
\item For any fixed \(h\in \mathcal{H}\) and \(\epsilon > 0\):
\begin{equation*}
\mathrm{Pr}[|\hat{L}(h)-L(h)|\leq \epsilon] \geq 1 - 2e^{-2n\epsilon^2}
\end{equation*}
\item For any \(\epsilon > 0\):
\begin{equation*}
\mathrm{Pr}[\forall h\in \mathcal{H}, | \hat{L}(h) - L(h)| \leq \epsilon]\geq 1 - 2|\mathcal{H}|e^{-2n\epsilon^2}
\end{equation*}
\end{enumerate}
\end{document}